ROOT
@@ -1,7 +1,8 @@
-session "Banks" in "Banks" = "UTP2" +
+session "Banks" in "Banks" = "UTP-Designs" +
     theories "./banks"
 
 session "BanksExamples" in "examples" = "Banks" + 
 theories
     "localise_globalise"
     "alice_guessing"
+    "byte_register"
